Complete adequacy with laters.

src/heaplang/adequacy.v
@@ -4,7 +4,7 @@ From iris Require Import invariants ghost_map.
 From iris.proofmode Require Import proofmode.
 From ITree Require Import ITree Recursion RecursionFacts InterpFacts Eqit.
 From iris.program_logic Require Import language.
-From iris.itree Require Import later.
+From iris.itree Require Import later handler.
 From iris.itree.threadpool Require Import handler interleaving.
 From iris.itree.heaplang Require Import lang.
 From Paco Require Import paco.
@@ -22,28 +22,28 @@ Proof.
   - right. intros Heq. by injection Heq as -> ->.
 Qed.
 
-Lemma compile_Fork {R} lt e (k : val → itree heaplangE R) :
-  (v ← compile_expr lt (Fork e) ; k v)%itree ≈ vis EFork (λ thread,
+Lemma compile_Fork {R} e (k : val → itree heaplangE R) :
+  (v ← compile_expr (Fork e) ; k v)%itree ≈ vis EFork (λ thread,
     match thread with
-    | CurrentThread => k (LitV LitUnit)
+    | CurrentThread => step ;; k (LitV LitUnit)
     | NewThread =>
-        v ← compile_expr lt e;
-        step_if_not_val lt e;;
+        v ← compile_expr e;
+        yield_if_not_val e;;
         kill_thread
     end
   )%itree.
 Proof.
-  rewrite /compile_expr. simpl_itree. simpl_itree.
+  rewrite /compile_expr. eutt_norm. simpl_itree.
   rewrite -bind_trigger. f_equiv. intros [|].
   - by simpl_itree.
   - simpl_itree. f_equiv. intros v. rewrite /kill_thread.
     f_equiv. intros _. rewrite -bind_trigger. f_equiv; first done. intros [].
 Qed.
 
-Lemma trace_base_Fork {R} lt tid (tp : list (itree heaplangE R)) tr e k :
-  tp !! tid = Some (v ← compile_expr lt (Fork e) ; k v)%itree →
-  is_ctrace tr tid (<[tid := k (LitV LitUnit)]>tp ++ [(compile_expr lt e ;; step_if_not_val lt e ;; kill_thread)%itree]) →
-  is_ctrace (CTFork (compile_expr lt e ;; step_if_not_val lt e ;; kill_thread) tr) tid tp.
+Lemma trace_base_Fork {R} tid (tp : list (itree heaplangE R)) tr e k :
+  tp !! tid = Some (v ← compile_expr (Fork e) ; k v)%itree →
+  is_ctrace tr tid (<[tid := (step ;; k (LitV LitUnit))%itree]>tp ++ [(compile_expr e ;; yield_if_not_val e ;; kill_thread)%itree]) →
+  is_ctrace (CTFork (compile_expr e ;; yield_if_not_val e ;; kill_thread) tr) tid tp.
 Proof.
   intros Htp Htr. eapply is_ctrace_insert; first done; first apply compile_Fork; eauto.
   eexists. split. { rewrite list_lookup_insert //. by apply lookup_lt_is_Some_1. }
@@ -56,66 +56,66 @@ Proof.
   by injection Ht' as <-.
 Qed.
 
-Lemma base_UnOp lt op v v' :
+Lemma base_UnOp op v v' :
   un_op_eval op v = Some v' →
-  compile_expr lt (UnOp op (Val v)) ≈ Ret v'.
+  compile_expr (UnOp op (Val v)) ≈ step_ret v'.
 Proof.
   intros Hop.
   rewrite /compile_expr. simpl_itree. rewrite Hop. by simpl_itree.
 Qed.
 
-Lemma base_BinOp lt op v1 v2 v3 :
+Lemma base_BinOp op v1 v2 v3 :
   bin_op_eval op v1 v2 = Some v3 →
-  compile_expr lt (BinOp op (Val v1) (Val v2)) ≈ Ret v3.
+  compile_expr (BinOp op (Val v1) (Val v2)) ≈ step_ret v3.
 Proof.
   intros Hop.
   rewrite /compile_expr. simpl_itree. rewrite Hop. by simpl_itree.
 Qed.
 
-Lemma base_Beta lt f_ x_ e v :
-  compile_expr lt (App (Val (RecV f_ x_ e)) (Val v))
+Lemma base_Beta f_ x_ e v :
+  compile_expr (App (Val (RecV f_ x_ e)) (Val v))
   ≈ let e' := (subst' x_ v (subst' f_ (RecV f_ x_ e) e))
-     in step_if_not_val lt e' ;; compile_expr lt e'.
+     in step_if_not_val e' ;; yield_if_not_val e' ;; compile_expr e'.
 Proof.
   rewrite /compile_expr. by simpl_itree.
 Qed.
 
-Definition compile_tp' lt (tp : list expr) : list (itree heaplangE val) :=
+Definition compile_tp' (tp : list expr) : list (itree heaplangE val) :=
   map (λ e,
-    compile_expr lt e ;;
-    step_if_not_val lt e ;;
+    compile_expr e ;;
+    yield_if_not_val e ;;
     kill_thread
   )%itree tp.
-Definition compile_tp lt (tp : list expr) : list (itree heaplangE val) :=
+Definition compile_tp (tp : list expr) : list (itree heaplangE val) :=
   map (λ '(tid, e),
-    v ← compile_expr lt e ;
-    step_if_not_val lt e ;;
+    v ← compile_expr e ;
+    yield_if_not_val e ;;
     match tid with
     | 0 => Ret v
     | _ => kill_thread
     end
   )%itree (enumerate tp).
 
-Lemma compile_tp_len lt tp :
-  length (compile_tp lt tp) = length tp.
+Lemma compile_tp_len tp :
+  length (compile_tp tp) = length tp.
 Proof. rewrite /compile_tp map_length enumerate_length //. Qed.
-Lemma compile_tp'_app lt tp tp' :
-  compile_tp' lt (tp ++ tp') = compile_tp' lt tp ++ compile_tp' lt tp'.
+Lemma compile_tp'_app tp tp' :
+  compile_tp' (tp ++ tp') = compile_tp' tp ++ compile_tp' tp'.
 Proof. rewrite /compile_tp' map_app //. Qed.
-Lemma compile_tp'_cons lt e tp :
-  compile_tp' lt (e :: tp) = compile_tp' lt [e] ++ compile_tp' lt tp.
+Lemma compile_tp'_cons e tp :
+  compile_tp' (e :: tp) = compile_tp' [e] ++ compile_tp' tp.
 Proof. done. Qed.
-Lemma compile_tp_cons lt e tp :
-  compile_tp lt (e :: tp) = compile_tp lt [e] ++ compile_tp' lt tp.
+Lemma compile_tp_cons e tp :
+  compile_tp (e :: tp) = compile_tp [e] ++ compile_tp' tp.
 Proof.
   rewrite /compile_tp /=. f_equiv.
   replace 1 with (S 0) by done.
   generalize 0. induction tp as [|e' tp IH]; first done. intros n.
   simpl. f_equiv. apply IH.
 Qed.
-Lemma compile_tp_app lt tp tp' :
+Lemma compile_tp_app tp tp' :
   length tp ≠ 0 →
-  compile_tp lt (tp ++ tp') = compile_tp lt tp ++ compile_tp' lt tp'.
+  compile_tp (tp ++ tp') = compile_tp tp ++ compile_tp' tp'.
 Proof.
   destruct tp as [|e tp]; first done. intros _.
   rewrite compile_tp_cons /= compile_tp_cons /= compile_tp'_app //.
@@ -476,21 +476,15 @@ Definition trace_invariant_postfix tp' σ' (tr : ctrace (demonicE +' stateE stat
   | Some tx => ctrace_terminates_in tr tx
   | None => False
   end.
-Fixpoint no_laters {R} (tr : trace (laterE +' ubE) R) : bool :=
-  match tr with
-  | TVis _ (inl1 ELater) _ _ => false
-  | TVis _ _ _ tr' => no_laters tr'
-  | _ => true
-  end.
-Definition trace_invariant_state (lt : bool) σ (tr : ctrace (demonicE +' stateE state +' laterE +' ubE) val) :=
-  match interp_tr_state σ (interp_tr (sequencify tr)) with
-  | Some tr' => no_laters tr' || lt
+Definition trace_invariant_state σ (tr : ctrace (demonicE +' stateE state +' laterE +' ubE) val) :=
+  match (interp_tr_state σ (interp_tr (sequencify tr))) with
+  | Some _ => true
   | None => false
   end.
 (* TODO: Add invariant about the final state reached in trace. Should be σ'. *)
-Definition trace_invariant (lt : bool) σ tp' σ' (tr : ctrace (demonicE +' stateE state +' laterE +' ubE) val) :=
+Definition trace_invariant σ tp' σ' (tr : ctrace (demonicE +' stateE state +' laterE +' ubE) val) :=
   trace_invariant_postfix tp' σ' tr ∧
-  trace_invariant_state lt σ tr.
+  trace_invariant_state σ tr.
 
 Lemma trace_invariant_postfix_postfix tp' σ' tr tr' :
   is_postfix_ctrace tr tr' →
@@ -519,9 +513,9 @@ Proof.
     destruct (decide _) as [Hstuck|]; try discriminate; rewrite -Heq //.
 Qed.
 
-Lemma is_ctrace_ret lt tp σ v :
+Lemma is_ctrace_ret tp σ v :
   tp_termination tp σ = Some (TermRet v) →
-  is_ctrace (CTRet v) 0 (compile_tp lt tp).
+  is_ctrace (CTRet v) 0 (compile_tp tp).
 Proof.
   intros Hterm.
   rewrite /tp_termination in Hterm.
@@ -533,9 +527,9 @@ Proof.
     exists (Ret v). split; first done. constructor.
 Qed.
 
-Lemma trace_invariant_ret lt tp σ v :
+Lemma trace_invariant_ret tp σ v :
   tp_termination tp σ = Some (TermRet v) →
-  trace_invariant lt σ tp σ (CTRet v).
+  trace_invariant σ tp σ (CTRet v).
 Proof.
   intros Hterm.
   rewrite /tp_termination in Hterm.
@@ -584,36 +578,39 @@ Lemma enumerate_lookup' {A} (xs : list A) (idx : nat) :
   (enumerate xs) !! idx = (λ x, (idx, x)) <$> (xs !! idx).
 Proof. apply enumerate_from_lookup'. Qed.
 
-Definition ctrace_step (lt : bool) (tid : nat) (tr : ctrace (demonicE +' stateE state +' laterE +' ubE) val) :=
-  if lt then CTVis () (subevent _ ELater) () (CTYield tid tr) else CTYield tid tr.
-Lemma is_ctrace_step lt tid tid' tp tr t :
-  tp !! tid = Some (ITree.bind (step lt) (λ _, t))%itree →
+Definition ctrace_step_yield (tid : nat) (tr : ctrace (demonicE +' stateE state +' laterE +' ubE) val) :=
+  CTVis () (subevent _ ELater) () (CTYield tid tr).
+Lemma is_ctrace_step_yield tid tid' tp tr t :
+  tp !! tid = Some (step ;; yield ;; t)%itree →
   is_ctrace tr tid' (<[tid := t]>tp) →
-  is_ctrace (ctrace_step lt tid' tr) tid tp.
+  is_ctrace (ctrace_step_yield tid' tr) tid tp.
 Proof.
-  intros Htp Htr. rewrite /ctrace_step. rewrite step_unfold in Htp. destruct lt.
-  - eapply is_ctrace_insert; first done. { simpl_itree. reflexivity. }
-    eapply is_ctrace_Vis.
-    { rewrite list_lookup_insert //. by apply lookup_lt_is_Some. }
-    rewrite list_insert_insert.
-    eapply is_ctrace_yield.
-    { rewrite list_lookup_insert //. by apply lookup_lt_is_Some. }
-    by rewrite list_insert_insert.
-  - eapply is_ctrace_insert; first done. { simpl_itree. reflexivity. }
-    eapply is_ctrace_yield.
-    { rewrite list_lookup_insert //. by apply lookup_lt_is_Some. }
-    by rewrite list_insert_insert.
+  intros Htp Htr. rewrite /ctrace_step_yield.
+  eapply is_ctrace_insert; first done. { simpl_itree. reflexivity. }
+  eapply is_ctrace_Vis.
+  { rewrite list_lookup_insert //. by apply lookup_lt_is_Some. }
+  rewrite list_insert_insert.
+  eapply is_ctrace_yield.
+  { rewrite list_lookup_insert //. by apply lookup_lt_is_Some. }
+  by rewrite list_insert_insert.
 Qed.
 
-Lemma state_invariant_step lt tid σ tr :
-  trace_invariant_state lt σ tr →
-  trace_invariant_state lt σ (ctrace_step lt tid tr).
+Lemma state_invariant_yield tid σ tr :
+  trace_invariant_state σ tr →
+  trace_invariant_state σ (CTYield tid tr).
 Proof.
   intros Hinv.
   rewrite /trace_invariant_state. rewrite /trace_invariant_state in Hinv.
-  destruct lt.
-  - rewrite /ctrace_step /=. by destruct (interp_tr_state _ _).
-  - done.
+  rewrite /ctrace_step_yield /=. by destruct (interp_tr_state _ _).
+Qed.
+
+Lemma state_invariant_step_yield tid σ tr :
+  trace_invariant_state σ tr →
+  trace_invariant_state σ (ctrace_step_yield tid tr).
+Proof.
+  intros Hinv.
+  rewrite /trace_invariant_state. rewrite /trace_invariant_state in Hinv.
+  rewrite /ctrace_step_yield /=. by destruct (interp_tr_state _ _).
 Qed.
 
 Definition ctrace_store' l x σ (tr : ctrace (demonicE +' stateE state +' laterE +' ubE) val) :=
@@ -718,32 +715,32 @@ Proof.
     { rewrite list_lookup_insert //. by apply lookup_lt_is_Some. }
 Qed.
 
-Lemma state_invariant_store' lt l x σ tr :
-  trace_invariant_state lt (state_upd_heap <[l:=x]> σ) tr →
-  trace_invariant_state lt σ (ctrace_store' l x σ tr).
+Lemma state_invariant_store' l x σ tr :
+  trace_invariant_state (state_upd_heap <[l:=x]> σ) tr →
+  trace_invariant_state σ (ctrace_store' l x σ tr).
 Proof.
   intros Hinv.
   rewrite /trace_invariant_state. rewrite /trace_invariant_state in Hinv.
   simpl. rewrite decide_True //.
 Qed.
-Lemma state_invariant_store lt l x σ tr :
-  trace_invariant_state lt (state_upd_heap <[l:=Some x]> σ) tr →
-  trace_invariant_state lt σ (ctrace_store l x σ tr).
+Lemma state_invariant_store l x σ tr :
+  trace_invariant_state (state_upd_heap <[l:=Some x]> σ) tr →
+  trace_invariant_state σ (ctrace_store l x σ tr).
 Proof.
   intros Hinv. by apply state_invariant_store'.
 Qed.
-Lemma state_invariant_load lt σ tr :
-  trace_invariant_state lt σ tr →
-  trace_invariant_state lt σ (ctrace_load σ tr).
+Lemma state_invariant_load σ tr :
+  trace_invariant_state σ tr →
+  trace_invariant_state σ (ctrace_load σ tr).
 Proof.
   intros Hinv.
   rewrite /trace_invariant_state. rewrite /trace_invariant_state in Hinv.
   simpl. rewrite decide_True //.
 Qed.
 
-Lemma stuck_ub lt tp σ :
+Lemma stuck_ub tp σ :
   tp_termination tp σ = Some TermUb →
-  ∃ tid tr, trace_invariant lt σ tp σ tr ∧ is_ctrace tr tid (compile_tp lt tp).
+  ∃ tid tr, trace_invariant σ tp σ tr ∧ is_ctrace tr tid (compile_tp tp).
 Proof.
   intros Hterm.
   assert (Hterm' := Hterm).
@@ -1180,187 +1177,196 @@ Lemma AllocN_free_locations n v σ ρs l efs :
   ∃ (l' : free_locations n σ), `l' = l.
 Proof. intros Hbase. by exists (to_free_location n v σ ρs l efs Hbase). Qed.
 
-Lemma step_in_thread lt e1 σ1 κs e2 σ2 efs tr tid tid' tp (k : val → itree heaplangE val) tp' σ' :
+Lemma step_in_thread e1 σ1 κs e2 σ2 efs tr tid tid' tp (k : val → itree heaplangE val) tp' σ' :
   base_step e1 σ1 κs e2 σ2 efs →
-  is_ctrace tr tid' (<[tid:=(v ← compile_expr lt e2 ; step_if_not_val lt e2 ;; k v)%itree]>tp
-                    ++ compile_tp' lt efs) →
-  trace_invariant lt σ2 tp' σ' tr →
-  tp !! tid = Some (v ← compile_expr lt e1 ; step_if_not_val lt e1 ;; k v)%itree →
-  ∃ tr', trace_invariant lt σ1 tp' σ' tr' ∧ is_ctrace tr' tid tp.
+  is_ctrace tr tid' (<[tid:=(v ← compile_expr e2 ; yield_if_not_val e2 ;; k v)%itree]>tp
+                    ++ compile_tp' efs) →
+  trace_invariant σ2 tp' σ' tr →
+  tp !! tid = Some (v ← compile_expr e1 ; yield_if_not_val e1 ;; k v)%itree →
+  ∃ tr', trace_invariant σ1 tp' σ' tr' ∧ is_ctrace tr' tid tp.
 Proof.
   intros Hbase Htr (Hub&Hstinv) Htp.
   inversion Hbase; subst; simpl in Htr; rewrite ?app_nil_r in Htr.
-  - exists (ctrace_step lt tid' tr). repeat split.
+  - exists (ctrace_step_yield tid' tr). repeat split.
     { apply trace_invariant_postfix_postfix with (tr := tr); eauto.
-      destruct lt; repeat constructor. }
-    { by apply state_invariant_step. }
+      repeat constructor. }
+    { by apply state_invariant_step_yield. }
     eapply is_ctrace_insert; first done.
-    { rewrite /compile_expr /step_if_not_val. simpl_itree. reflexivity. }
-    apply is_ctrace_step with (t := k (RecV f x e)).
+    { rewrite /compile_expr. simpl_itree. reflexivity. }
+    apply is_ctrace_step_yield with (t := k (RecV f x e)).
     { rewrite list_lookup_insert //. by apply lookup_lt_is_Some. }
     rewrite list_insert_insert.
     by simpl_itree in Htr.
-  - exists (ctrace_step lt tid' tr). repeat split.
+  - exists (ctrace_step_yield tid' tr). repeat split.
     { apply trace_invariant_postfix_postfix with (tr := tr); eauto.
-      destruct lt; repeat constructor. }
-    { by apply state_invariant_step. }
+      repeat constructor. }
+    { by apply state_invariant_step_yield. }
     eapply is_ctrace_insert; first done.
     { rewrite /= /compile_expr. simpl_itree. reflexivity. }
-    apply is_ctrace_step with (t := k (PairV v1 v2)).
+    apply is_ctrace_step_yield with (t := k (PairV v1 v2)).
     { rewrite list_lookup_insert //. by apply lookup_lt_is_Some. }
     rewrite list_insert_insert.
     by simpl_itree in Htr.
-  - exists (ctrace_step lt tid' tr). repeat split.
+  - exists (ctrace_step_yield tid' tr). repeat split.
     { apply trace_invariant_postfix_postfix with (tr := tr); eauto.
-      destruct lt; repeat constructor. }
-    { by apply state_invariant_step. }
+      repeat constructor. }
+    { by apply state_invariant_step_yield. }
     eapply is_ctrace_insert; first done.
     { rewrite /= /compile_expr. simpl_itree. reflexivity. }
-    apply is_ctrace_step with (t := k (InjLV v)).
+    apply is_ctrace_step_yield with (t := k (InjLV v)).
     { rewrite list_lookup_insert //. by apply lookup_lt_is_Some. }
     rewrite list_insert_insert.
     by simpl_itree in Htr.
-  - exists (ctrace_step lt tid' tr). repeat split.
+  - exists (ctrace_step_yield tid' tr). repeat split.
     { apply trace_invariant_postfix_postfix with (tr := tr); eauto.
-      destruct lt; repeat constructor. }
-    { by apply state_invariant_step. }
+      repeat constructor. }
+    { by apply state_invariant_step_yield. }
     eapply is_ctrace_insert; first done.
     { rewrite /= /compile_expr. simpl_itree. reflexivity. }
-    apply is_ctrace_step with (t := k (InjRV v)).
+    apply is_ctrace_step_yield with (t := k (InjRV v)).
     { rewrite list_lookup_insert //. by apply lookup_lt_is_Some. }
     rewrite list_insert_insert.
     by simpl_itree in Htr.
   - pose (e' := subst' x v2 (subst' f (RecV f x e0) e0)).
-    exists (ctrace_step lt tid' tr). repeat split.
-    { apply trace_invariant_postfix_postfix with (tr := tr); eauto.
-      destruct lt; repeat constructor. }
-    { by apply state_invariant_step. }
     destruct (to_val e') as [v|] eqn:Hval.
-    * eapply is_ctrace_insert; first done.
-      { rewrite /= base_Beta /= /step_if_not_val.
+    * exists (CTYield tid' tr). repeat split.
+      { apply trace_invariant_postfix_postfix with (tr := tr); eauto.
+        repeat constructor. }
+      { by apply state_invariant_yield. }
+      eapply is_ctrace_insert; first done.
+      { rewrite /= base_Beta /= /step_if_not_val /yield_if_not_val.
         rewrite /e' in Hval. rewrite Hval. rewrite bind_ret_l.
-        reflexivity. }
+        simpl_itree. reflexivity. }
       rewrite /e' in Hval. apply of_to_val in Hval as Heq.
-      rewrite -Heq in Htr. rewrite -Heq.
-      rewrite compile_expr_val. rewrite compile_expr_val in Htr.
-      simpl in Htr.
-      rewrite bind_ret_l. rewrite !bind_ret_l in Htr.
-      apply is_ctrace_step with (t := k v).
+      rewrite -Heq in Htr. rewrite -Heq. simpl_itree. simpl_itree in Htr.
+      apply is_ctrace_yield with (t := k v).
       { rewrite list_lookup_insert //. by apply lookup_lt_is_Some. }
       by rewrite list_insert_insert.
-    * eapply is_ctrace_insert; first done.
-      { rewrite /= base_Beta /= /step_if_not_val. rewrite /e' in Hval.
+    * exists (ctrace_step_yield tid' tr). repeat split.
+      { apply trace_invariant_postfix_postfix with (tr := tr); eauto.
+        repeat constructor. }
+      { by apply state_invariant_step_yield. }
+      eapply is_ctrace_insert; first done.
+      { rewrite /= base_Beta /= /yield_if_not_val /step_if_not_val. rewrite /e' in Hval.
         rewrite Hval. reflexivity. }
-      rewrite /e' in Hval. rewrite /step_if_not_val in Htr. rewrite Hval in Htr.
-      rewrite bind_bind.
-      apply is_ctrace_step with (t := (v ← compile_expr lt e'; step lt ;; k v)%itree).
+      rewrite /e' in Hval. rewrite /yield_if_not_val /step_if_not_val in Htr. rewrite Hval in Htr.
+      rewrite bind_bind. setoid_rewrite bind_bind.
+      apply is_ctrace_step_yield with (t := (v ← compile_expr e'; yield ;; k v)%itree).
       { rewrite list_lookup_insert //. by apply lookup_lt_is_Some. }
       by rewrite list_insert_insert.
-  - exists (ctrace_step lt tid' tr). repeat split.
+  - exists (ctrace_step_yield tid' tr). repeat split.
     { apply trace_invariant_postfix_postfix with (tr := tr); eauto.
-      destruct lt; repeat constructor. }
-    { by apply state_invariant_step. }
+      repeat constructor. }
+    { by apply state_invariant_step_yield. }
     rewrite compile_expr_val !bind_ret_l in Htr.
-    eapply is_ctrace_insert with (t' := (step lt ;; k v')%itree); first done.
-    { rewrite base_UnOp // bind_ret_l  //. }
-    eapply is_ctrace_step. { rewrite list_lookup_insert //. by apply lookup_lt_is_Some. }
+    eapply is_ctrace_insert with (t' := (step ;; yield ;; k v')%itree); first done.
+    { rewrite base_UnOp //. by simpl_itree. }
+    eapply is_ctrace_step_yield. { rewrite list_lookup_insert //. by apply lookup_lt_is_Some. }
     by rewrite list_insert_insert.
-  - exists (ctrace_step lt tid' tr). repeat split.
+  - exists (ctrace_step_yield tid' tr). repeat split.
     { apply trace_invariant_postfix_postfix with (tr := tr); eauto.
-      destruct lt; repeat constructor. }
-    { by apply state_invariant_step. }
+      repeat constructor. }
+    { by apply state_invariant_step_yield. }
     rewrite compile_expr_val !bind_ret_l in Htr.
-    eapply is_ctrace_insert with (t' := (step lt ;; k v')%itree); first done.
-    { rewrite base_BinOp // bind_ret_l  //. }
-    eapply is_ctrace_step. { rewrite list_lookup_insert //. by apply lookup_lt_is_Some. }
+    eapply is_ctrace_insert with (t' := (step ;; yield ;; k v')%itree); first done.
+    { rewrite base_BinOp //. by simpl_itree. }
+    eapply is_ctrace_step_yield. { rewrite list_lookup_insert //. by apply lookup_lt_is_Some. }
     by rewrite list_insert_insert.
-  - exists (ctrace_step lt tid' tr). repeat split.
-    { apply trace_invariant_postfix_postfix with (tr := tr); eauto.
-      destruct lt; repeat constructor. }
-    { by apply state_invariant_step. }
-    destruct (to_val e2) eqn:Hval.
-    * apply of_to_val in Hval as <-.
+  - destruct (to_val e2) eqn:Hval.
+    * exists (CTYield tid' tr). repeat split.
+      { apply trace_invariant_postfix_postfix with (tr := tr); eauto.
+        repeat constructor. }
+      { by apply state_invariant_yield. }
+      apply of_to_val in Hval as <-.
       eapply is_ctrace_insert; first done.
       { rewrite /= /compile_expr. simpl_itree. reflexivity. }
-      apply is_ctrace_step with (t := k v).
+      apply is_ctrace_yield with (t := k v).
       { rewrite list_lookup_insert //. by apply lookup_lt_is_Some. }
       rewrite list_insert_insert.
       by simpl_itree in Htr.
-    * eapply is_ctrace_insert; first done.
+    * exists (ctrace_step_yield tid' tr). repeat split.
+      { apply trace_invariant_postfix_postfix with (tr := tr); eauto.
+        repeat constructor. }
+      { by apply state_invariant_step_yield. }
+      eapply is_ctrace_insert; first done.
       { rewrite /compile_expr. simpl_itree.
-        rewrite /step_if_not_val Hval /=. reflexivity. }
-      rewrite /step_if_not_val Hval in Htr. simpl_itree in Htr.
-      eapply is_ctrace_step.
+        rewrite /yield_if_not_val /step_if_not_val Hval /=. reflexivity. }
+      rewrite /yield_if_not_val Hval in Htr. simpl_itree in Htr.
+      eapply is_ctrace_step_yield.
       { rewrite list_lookup_insert //. by apply lookup_lt_is_Some. }
       rewrite list_insert_insert.
       by simpl_itree in Htr.
-  - exists (ctrace_step lt tid' tr). repeat split.
-    { apply trace_invariant_postfix_postfix with (tr := tr); eauto.
-      destruct lt; repeat constructor. }
-    { by apply state_invariant_step. }
-    destruct (to_val e2) eqn:Hval.
-    * apply of_to_val in Hval as <-.
+  - destruct (to_val e2) eqn:Hval.
+    * exists (CTYield tid' tr). repeat split.
+      { apply trace_invariant_postfix_postfix with (tr := tr); eauto.
+        repeat constructor. }
+      { by apply state_invariant_yield. }
+      apply of_to_val in Hval as <-.
       eapply is_ctrace_insert; first done.
       { rewrite /compile_expr. simpl_itree.
         rewrite /step_if_not_val /=. reflexivity. }
-      apply is_ctrace_step with (t := k v).
+      apply is_ctrace_yield with (t := k v).
       { rewrite list_lookup_insert //. by apply lookup_lt_is_Some. }
       rewrite list_insert_insert.
       by simpl_itree in Htr.
-    * eapply is_ctrace_insert; first done.
+    * exists (ctrace_step_yield tid' tr). repeat split.
+      { apply trace_invariant_postfix_postfix with (tr := tr); eauto.
+        repeat constructor. }
+      { by apply state_invariant_step_yield. }
+      eapply is_ctrace_insert; first done.
       { simpl. rewrite /compile_expr. simpl_itree.
-        rewrite /step_if_not_val Hval /=. reflexivity. }
-      rewrite /step_if_not_val Hval in Htr. simpl_itree in Htr.
-      eapply is_ctrace_step.
+        rewrite /yield_if_not_val /step_if_not_val Hval /=. reflexivity. }
+      rewrite /yield_if_not_val Hval in Htr. simpl_itree in Htr.
+      eapply is_ctrace_step_yield.
       { rewrite list_lookup_insert //. by apply lookup_lt_is_Some. }
       rewrite list_insert_insert.
       by simpl_itree in Htr.
-  - exists (ctrace_step lt tid' tr). repeat split.
+  - exists (ctrace_step_yield tid' tr). repeat split.
     { apply trace_invariant_postfix_postfix with (tr := tr); eauto.
-      destruct lt; repeat constructor. }
-    { by apply state_invariant_step. }
+      repeat constructor. }
+    { by apply state_invariant_step_yield. }
     rewrite compile_expr_val !bind_ret_l in Htr.
-    eapply is_ctrace_insert with (t' := (step lt ;; k v1)%itree); first done.
+    eapply is_ctrace_insert with (t' := (step ;; yield ;; k v1)%itree); first done.
     { rewrite /compile_expr. simpl_itree. reflexivity. }
-    eapply is_ctrace_step. { rewrite list_lookup_insert //. by apply lookup_lt_is_Some. }
+    eapply is_ctrace_step_yield. { rewrite list_lookup_insert //. by apply lookup_lt_is_Some. }
     by rewrite list_insert_insert.
-  - exists (ctrace_step lt tid' tr). repeat split.
+  - exists (ctrace_step_yield tid' tr). repeat split.
     { apply trace_invariant_postfix_postfix with (tr := tr); eauto.
-      destruct lt; repeat constructor. }
-    { by apply state_invariant_step. }
+      repeat constructor. }
+    { by apply state_invariant_step_yield. }
     rewrite compile_expr_val !bind_ret_l in Htr.
-    eapply is_ctrace_insert with (t' := (step lt ;; k v2)%itree); first done.
+    eapply is_ctrace_insert with (t' := (step ;; yield ;; k v2)%itree); first done.
     { rewrite /compile_expr. simpl_itree. reflexivity. }
-    eapply is_ctrace_step. { rewrite list_lookup_insert //. by apply lookup_lt_is_Some. }
+    eapply is_ctrace_step_yield. { rewrite list_lookup_insert //. by apply lookup_lt_is_Some. }
     by rewrite list_insert_insert.
-  - exists (ctrace_step lt tid' tr). repeat split.
+  - exists (ctrace_step_yield tid' tr). repeat split.
     { apply trace_invariant_postfix_postfix with (tr := tr); eauto.
-      destruct lt; repeat constructor. }
-    { by apply state_invariant_step. }
+      repeat constructor. }
+    { by apply state_invariant_step_yield. }
     eapply is_ctrace_insert; first done.
     { simpl. rewrite /compile_expr. simpl_itree.
       rewrite /step_if_not_val /=. reflexivity. }
-    eapply is_ctrace_step.
+    eapply is_ctrace_step_yield.
     { rewrite list_lookup_insert //. by apply lookup_lt_is_Some. }
     rewrite list_insert_insert.
     by simpl_itree in Htr.
-  - exists (ctrace_step lt tid' tr). repeat split.
+  - exists (ctrace_step_yield tid' tr). repeat split.
     { apply trace_invariant_postfix_postfix with (tr := tr); eauto.
-      destruct lt; repeat constructor. }
-    { by apply state_invariant_step. }
+      repeat constructor. }
+    { by apply state_invariant_step_yield. }
     eapply is_ctrace_insert; first done.
     { simpl. rewrite /compile_expr. simpl_itree.
-      rewrite /step_if_not_val /=. reflexivity. }
-    eapply is_ctrace_step.
+      rewrite /yield_if_not_val /=. reflexivity. }
+    eapply is_ctrace_step_yield.
     { rewrite list_lookup_insert //. by apply lookup_lt_is_Some. }
     rewrite list_insert_insert.
     by simpl_itree in Htr.
   - destruct (AllocN_free_locations _ _ _ _ _ _ Hbase) as [ll <-].
-    exists (CTVis state (subevent _ EGetState) σ1 (CTVis (free_locations n σ1) (subevent _ (EDemonic (free_locations n σ1))) ll (CTVis () (subevent _ (ESetState (state_init_heap (`ll) n v σ1))) () (ctrace_step lt tid' tr)))).
+    exists (CTVis state (subevent _ EGetState) σ1 (CTVis (free_locations n σ1) (subevent _ (EDemonic (free_locations n σ1))) ll (CTVis () (subevent _ (ESetState (state_init_heap (`ll) n v σ1))) () (ctrace_step_yield tid' tr)))).
     repeat split.
     { apply trace_invariant_postfix_postfix with (tr := tr); eauto.
-      destruct lt; repeat constructor. }
-    { rewrite /trace_invariant_state /= decide_True //. by apply state_invariant_step. }
+      repeat constructor. }
+    { rewrite /trace_invariant_state /= decide_True //. by apply state_invariant_step_yield. }
     eapply is_ctrace_insert; first done.
     { simpl. rewrite /compile_expr. simpl_itree. reflexivity. }
     rewrite assert_True; last lia. simpl_itree.
@@ -1372,58 +1378,58 @@ Proof.
     eapply is_ctrace_Vis.
     { rewrite list_insert_insert list_lookup_insert // insert_length -lookup_lt_is_Some //. }
     rewrite !list_insert_insert.
-    eapply is_ctrace_step.
+    eapply is_ctrace_step_yield.
     { rewrite list_lookup_insert //. by apply lookup_lt_is_Some. }
     rewrite list_insert_insert.
     by simpl_itree in Htr.
-  - exists (ctrace_store' l None σ1 (ctrace_step lt tid' tr)). repeat split.
+  - exists (ctrace_store' l None σ1 (ctrace_step_yield tid' tr)). repeat split.
     { apply trace_invariant_postfix_postfix with (tr := tr); eauto.
-      destruct lt; repeat constructor. }
-    { rewrite /trace_invariant_state /= decide_True //. by apply state_invariant_step. }
+      repeat constructor. }
+    { rewrite /trace_invariant_state /= decide_True //. by apply state_invariant_step_yield. }
     eapply is_ctrace_insert; first done.
     { simpl. rewrite /compile_expr. simpl_itree. reflexivity. }
     eapply is_ctrace_store'; first done.
     { rewrite list_lookup_insert // -lookup_lt_is_Some //. }
-    eapply is_ctrace_step.
+    eapply is_ctrace_step_yield.
     { rewrite list_lookup_insert // insert_length. by apply lookup_lt_is_Some. }
     rewrite !list_insert_insert.
     by simpl_itree in Htr.
-  - exists (ctrace_load σ2 (ctrace_step lt tid' tr)). repeat split.
+  - exists (ctrace_load σ2 (ctrace_step_yield tid' tr)). repeat split.
     { apply trace_invariant_postfix_postfix with (tr := tr); eauto.
-      destruct lt; repeat constructor. }
-    { rewrite /trace_invariant_state /= decide_True //. by apply state_invariant_step. }
+      repeat constructor. }
+    { rewrite /trace_invariant_state /= decide_True //. by apply state_invariant_step_yield. }
     eapply is_ctrace_insert; first done.
     { simpl. rewrite /compile_expr. simpl_itree. reflexivity. }
     eapply is_ctrace_load; first done.
     { rewrite list_lookup_insert // -lookup_lt_is_Some //. }
     rewrite list_insert_insert.
-    eapply is_ctrace_step.
+    eapply is_ctrace_step_yield.
     { rewrite list_lookup_insert //. by apply lookup_lt_is_Some. }
     rewrite list_insert_insert.
     by simpl_itree in Htr.
-  - exists (ctrace_store l w σ1 (ctrace_step lt tid' tr)). repeat split.
+  - exists (ctrace_store l w σ1 (ctrace_step_yield tid' tr)). repeat split.
     { apply trace_invariant_postfix_postfix with (tr := tr); eauto.
-      destruct lt; repeat constructor. }
-    { rewrite /trace_invariant_state /= decide_True //. by apply state_invariant_step. }
+      repeat constructor. }
+    { rewrite /trace_invariant_state /= decide_True //. by apply state_invariant_step_yield. }
     eapply is_ctrace_insert; first done.
     { simpl. rewrite /compile_expr. simpl_itree. reflexivity. }
     eapply is_ctrace_store; first done.
     { rewrite list_lookup_insert // -lookup_lt_is_Some //. }
     rewrite !list_insert_insert.
-    eapply is_ctrace_step.
+    eapply is_ctrace_step_yield.
     { rewrite list_lookup_insert //. by apply lookup_lt_is_Some. }
     rewrite list_insert_insert.
     by simpl_itree in Htr.
-  - exists (ctrace_store l v2 σ1 (ctrace_step lt tid' tr)). repeat split.
+  - exists (ctrace_store l v2 σ1 (ctrace_step_yield tid' tr)). repeat split.
     { apply trace_invariant_postfix_postfix with (tr := tr); eauto.
-      destruct lt; repeat constructor. }
-    { rewrite /trace_invariant_state /= decide_True //. by apply state_invariant_step. }
+      repeat constructor. }
+    { rewrite /trace_invariant_state /= decide_True //. by apply state_invariant_step_yield. }
     eapply is_ctrace_insert; first done.
     { simpl. rewrite /compile_expr. simpl_itree. reflexivity. }
     eapply is_ctrace_store; first done.
     { rewrite list_lookup_insert // -lookup_lt_is_Some //. }
     rewrite !list_insert_insert.
-    eapply is_ctrace_step.
+    eapply is_ctrace_step_yield.
     { rewrite list_lookup_insert //. by apply lookup_lt_is_Some. }
     rewrite list_insert_insert.
     by simpl_itree in Htr.
@@ -1431,10 +1437,10 @@ Proof.
     * rewrite bool_decide_eq_true_2 // in Hstinv.
       rewrite bool_decide_eq_true_2 // in Hbase.
       rewrite bool_decide_eq_true_2 // in Htr.
-      exists (ctrace_load σ1 (ctrace_store l v2 σ1 (ctrace_step lt tid' tr))). repeat split.
+      exists (ctrace_load σ1 (ctrace_store l v2 σ1 (ctrace_step_yield tid' tr))). repeat split.
       { apply trace_invariant_postfix_postfix with (tr := tr); eauto.
-        destruct lt; repeat constructor. }
-      { rewrite /trace_invariant_state /= !decide_True //. by apply state_invariant_step. }
+        repeat constructor. }
+      { rewrite /trace_invariant_state /= !decide_True //. by apply state_invariant_step_yield. }
       eapply is_ctrace_insert; first done.
       { simpl. rewrite /compile_expr. simpl_itree. reflexivity. }
       eapply is_ctrace_load; first done.
@@ -1444,30 +1450,30 @@ Proof.
       eapply is_ctrace_store; first done.
       { rewrite list_lookup_insert // -lookup_lt_is_Some //. }
       rewrite !list_insert_insert.
-      eapply is_ctrace_step.
+      eapply is_ctrace_step_yield.
       { rewrite list_lookup_insert //. by apply lookup_lt_is_Some. }
       rewrite list_insert_insert.
       by simpl_itree in Htr.
     * rewrite bool_decide_eq_false_2 // in Hstinv.
       rewrite bool_decide_eq_false_2 // in Hbase.
       rewrite bool_decide_eq_false_2 // in Htr.
-      exists (ctrace_load σ1 (ctrace_step lt tid' tr)). repeat split.
+      exists (ctrace_load σ1 (ctrace_step_yield tid' tr)). repeat split.
       { apply trace_invariant_postfix_postfix with (tr := tr); eauto.
-        destruct lt; repeat constructor. }
-      { rewrite /trace_invariant_state /= !decide_True //. by apply state_invariant_step. }
+        repeat constructor. }
+      { rewrite /trace_invariant_state /= !decide_True //. by apply state_invariant_step_yield. }
       eapply is_ctrace_insert; first done.
       { simpl. rewrite /compile_expr. simpl_itree. reflexivity. }
       eapply is_ctrace_load; first done.
       { rewrite list_lookup_insert // -lookup_lt_is_Some //. }
       simpl. rewrite list_insert_insert. rewrite assert_True // decide_False //. simpl_itree.
-      eapply is_ctrace_step.
+      eapply is_ctrace_step_yield.
       { rewrite list_lookup_insert //. by apply lookup_lt_is_Some. }
       rewrite list_insert_insert.
       by simpl_itree in Htr.
-  - exists (ctrace_load σ1 (ctrace_store l (LitV (LitInt (i1 + i2))) σ1 (ctrace_step lt tid' tr))). repeat split.
+  - exists (ctrace_load σ1 (ctrace_store l (LitV (LitInt (i1 + i2))) σ1 (ctrace_step_yield tid' tr))). repeat split.
     { apply trace_invariant_postfix_postfix with (tr := tr); eauto.
-      destruct lt; repeat constructor. }
-    { rewrite /trace_invariant_state /= !decide_True //. by apply state_invariant_step. }
+      repeat constructor. }
+    { rewrite /trace_invariant_state /= !decide_True //. by apply state_invariant_step_yield. }
     eapply is_ctrace_insert; first done.
     { simpl. rewrite /compile_expr. simpl_itree. reflexivity. }
     eapply is_ctrace_load; first done.
@@ -1476,18 +1482,18 @@ Proof.
     eapply is_ctrace_store; first done.
     { rewrite list_lookup_insert // -lookup_lt_is_Some //. }
     rewrite list_insert_insert.
-    eapply is_ctrace_step.
+    eapply is_ctrace_step_yield.
     { rewrite list_lookup_insert //. by apply lookup_lt_is_Some. }
     rewrite list_insert_insert.
     by simpl_itree in Htr.
-  - exists (CTFork (compile_expr lt e ;; step_if_not_val lt e ;; kill_thread) (ctrace_step lt tid' tr)).
+  - exists (CTFork (compile_expr e ;; yield_if_not_val e ;; kill_thread) (ctrace_step_yield tid' tr)).
     repeat split.
     { apply trace_invariant_postfix_postfix with (tr := tr); eauto.
-      destruct lt; repeat constructor. }
-    { by apply state_invariant_step. }
+      repeat constructor. }
+    { by apply state_invariant_step_yield. }
     rewrite compile_expr_val !bind_ret_l in Htr.
     eapply trace_base_Fork; first apply Htp.
-    eapply is_ctrace_step.
+    eapply is_ctrace_step_yield.
     { rewrite lookup_app_l; last rewrite insert_length -lookup_lt_is_Some //.
       rewrite list_lookup_insert //. by apply lookup_lt_is_Some. }
     rewrite insert_app_l; last rewrite insert_length -lookup_lt_is_Some //.
@@ -1501,22 +1507,22 @@ Lemma lt_gt n m :
 Proof. lia. Qed.
 
 (* TODO: Idea: make κ = [] *)
-Lemma has_trace lt n tp σ tp' σ' κ tx :
+Lemma has_trace n tp σ tp' σ' κ tx :
   language.nsteps n (tp, σ) κ (tp', σ') →
   tp_termination tp' σ' = Some tx →
   length tp > 0 →
   ∃ tid tr,
-    trace_invariant lt σ tp' σ' tr ∧
-    is_ctrace (R := val) tr tid (compile_tp lt tp).
+    trace_invariant σ tp' σ' tr ∧
+    is_ctrace (R := val) tr tid (compile_tp tp).
 Proof.
   revert tp σ tp' σ' κ. induction n as [|n IH]; intros tp σ tp' σ' κ Hstep Hterm Hne.
   { destruct tx as [r|].
     - assert (Hterm' := Hterm).
-      apply is_ctrace_ret with (lt := lt) in Hterm as Htr.
-      apply trace_invariant_ret with (lt := lt) (σ := σ') in Hterm' as Htinv.
+      apply is_ctrace_ret  in Hterm as Htr.
+      apply trace_invariant_ret with (σ := σ') in Hterm' as Htinv.
       exists 0, (CTRet r). inversion Hstep. subst. by split.
     - inversion Hstep; subst.
-      apply stuck_ub with (lt := lt) in Hterm as (tid&tr&Hinv&Htr); eauto.
+      apply stuck_ub in Hterm as (tid&tr&Hinv&Htr); eauto.
   }
   inversion Hstep as [|m [tp1 σ1] [tp2 σ2] [tp3 σ3] ? ? Hstep'' Hstep']. subst.
   inversion Hstep'' as [e1' σ1 e2' σ2' efs tpa tpb Htp' Htp2' Hprim].
@@ -1534,14 +1540,14 @@ Proof.
     }
     destruct (decide (length tpa = 0)) as [Htpa|Htpa].
     * apply nil_length_inv in Htpa as ->. simpl. simpl in *.
-      apply step_in_thread with (lt := lt) (tp := ((v ← compile_expr lt e1; step_if_not_val lt e1;; Ret v)%itree :: compile_tp' lt tpb)) (tid := 0) (tid' := tid) (k := λ v, Ret v) (tr := tr) (tp' := tp') (σ' := σ') in Hbase as [tr' [Hinv' Htr']].
+      apply step_in_thread with (tp := ((v ← compile_expr e1; yield_if_not_val e1;; Ret v)%itree :: compile_tp' tpb)) (tid := 0) (tid' := tid) (k := λ v, Ret v) (tr := tr) (tp' := tp') (σ' := σ') in Hbase as [tr' [Hinv' Htr']].
       + exists 0, tr'. rewrite compile_tp_cons //.
       + simpl. rewrite compile_tp_cons compile_tp'_app // in Htr.
       + done.
       + done.
-    * apply step_in_thread with (lt := lt) (tp := (compile_tp lt tpa ++ (v ← compile_expr lt e1; step_if_not_val lt e1;; kill_thread)%itree :: compile_tp' lt tpb)) (tid := length (compile_tp lt tpa)) (tid' := tid) (k := λ v, kill_thread) (tr := tr) (tp' := tp') (σ' := σ') in Hbase as [tr' [Hinv' Htr']].
-      + exists (length (compile_tp lt tpa)), tr'. rewrite compile_tp_app //.
-      + replace (length (compile_tp lt tpa)) with (length (compile_tp lt tpa) + 0) by lia.
+    * apply step_in_thread with (tp := (compile_tp tpa ++ (v ← compile_expr e1; yield_if_not_val e1;; kill_thread)%itree :: compile_tp' tpb)) (tid := length (compile_tp tpa)) (tid' := tid) (k := λ v, kill_thread) (tr := tr) (tp' := tp') (σ' := σ') in Hbase as [tr' [Hinv' Htr']].
+      + exists (length (compile_tp tpa)), tr'. rewrite compile_tp_app //.
+      + replace (length (compile_tp tpa)) with (length (compile_tp tpa) + 0) by lia.
         rewrite compile_tp_app // in Htr.
         rewrite insert_app_r /= -app_assoc /=.
         rewrite compile_tp'_cons compile_tp'_app // in Htr.
@@ -1553,7 +1559,7 @@ Proof.
     }
     destruct (decide (length tpa = 0)) as [Htpa|Htpa].
     * apply nil_length_inv in Htpa as ->. simpl. simpl in *.
-      apply step_in_thread with (lt := lt) (tp := ((v ← compile_expr lt e1; step_if_not_val lt e1;; w ← compile_expr lt (fill K (Val v)); step lt;; Ret w)%itree :: compile_tp' lt tpb)) (tid := 0) (tid' := tid) (k := λ v, (w ← compile_expr lt (fill K (Val v)); step lt;; Ret w)%itree) (tr := tr) (tp' := tp') (σ' := σ') in Hbase as [tr' [Hinv' Htr']].
+      apply step_in_thread with (tp := ((v ← compile_expr e1; yield_if_not_val e1;; w ← compile_expr (fill K (Val v)); yield ;; Ret w)%itree :: compile_tp' tpb)) (tid := 0) (tid' := tid) (k := λ v, (w ← compile_expr (fill K (Val v)); yield ;; Ret w)%itree) (tr := tr) (tp' := tp') (σ' := σ') in Hbase as [tr' [Hinv' Htr']].
       + exists 0, tr'.
         split; first done.
         rewrite compile_tp_cons /= compile_expr_bind.
@@ -1572,7 +1578,7 @@ Proof.
       + done.
     * rewrite compile_tp_app // in Htr.
       rewrite compile_tp_app //.
-      apply step_in_thread with (lt := lt) (tp := (compile_tp lt tpa ++ (v ← compile_expr lt e1; step_if_not_val lt e1;; compile_expr lt (fill K (Val v));; step lt ;; kill_thread)%itree :: compile_tp' lt tpb)) (tid := length tpa) (tid' := tid) (k := λ v, (compile_expr lt (fill K (Val v));; step lt;; kill_thread)%itree) (tr := tr) (tp' := tp') (σ' := σ') in Hbase as [tr' [Hinv' Htr']].
+      apply step_in_thread with (tp := (compile_tp tpa ++ (v ← compile_expr e1; yield_if_not_val e1;; compile_expr (fill K (Val v));; yield ;; kill_thread)%itree :: compile_tp' tpb)) (tid := length tpa) (tid' := tid) (k := λ v, (compile_expr (fill K (Val v));; yield ;; kill_thread)%itree) (tr := tr) (tp' := tp') (σ' := σ') in Hbase as [tr' [Hinv' Htr']].
       + exists (length tpa), tr'.
         split; first done.
         rewrite /= compile_expr_bind.
@@ -1580,7 +1586,7 @@ Proof.
            rewrite bind_bind. by setoid_rewrite bind_bind.
         ++ admit.
         ++ rewrite -lt_gt -Nat.neq_0_lt_0 //.
-      + replace (length tpa) with (length (compile_tp lt tpa) + 0) by rewrite compile_tp_len //.
+      + replace (length tpa) with (length (compile_tp tpa) + 0) by rewrite compile_tp_len //.
         rewrite insert_app_r /= -app_assoc /=.
         rewrite compile_tp'_cons compile_tp'_app /= compile_expr_bind in Htr.
         ++ setoid_rewrite fill_not_val in Htr; last first. { rewrite -lt_gt -Nat.neq_0_lt_0 //. }
@@ -1666,22 +1672,56 @@ Proof.
   - inversion Hret.
 Qed.
 
+Inductive terminates_in' {R} : itree' (laterE +' ubE) R → Terminal R → Prop :=
+  | terminates_in_ELater tx k :
+  terminates_in' (observe (k ())) tx →
+  terminates_in' (VisF (inl1 ELater) k) tx
+  | terminates_in_Tau tx t :
+  terminates_in' (observe t) tx →
+  terminates_in' (TauF t) tx
+  | terminates_in_EUb k :
+  terminates_in' (VisF (inr1 EUb) k) TermUb
+  | terminates_in_Ret r :
+  terminates_in' (RetF r) (TermRet r).
+Definition terminates_in {R} (t : itree (laterE +' ubE) R) (tx : Terminal R) : Prop :=
+  terminates_in' (observe t) tx.
+Fixpoint model_terminal {R} (laters : nat) (tx : Terminal R) : itree (laterE +' ubE) R :=
+  match laters with
+  | O =>
+    match tx with
+    | TermRet r => Ret r
+    | TermUb => ub
+    end
+  | S n => step ;; model_terminal n tx
+  end.
+Lemma terminates_in_model {R} (t : itree (laterE +' ubE) R) tx :
+  terminates_in t tx →
+  ∃ n, t ≈ model_terminal n tx.
+Proof.
+  intros Hterm. rewrite /terminates_in in Hterm.
+  remember (observe t) as ot. revert t Heqot. induction Hterm; intros t' Heqot.
+  - destruct (IHHterm (k ())) as [n Heutt]; first done.
+    exists (S n). simplify_obs. simpl. rewrite bind_trigger.
+    f_equiv. f_equiv. by intros [].
+  - destruct (IHHterm t) as [n Heutt]; first done.
+    exists n. simplify_obs. by transitivity t; first by apply tau_eutt.
+  - exists 0. simplify_obs. simpl. rewrite /ub. f_equiv. f_equiv. intros [].
+  - exists 0. by simplify_obs.
+Qed.
+
 Lemma is_trace_term {R} (t : itree (laterE +' ubE) R) tr tx :
   trace_terminates_in tr tx →
   is_trace tr t →
-  no_laters tr →
-  t ≈ match tx with
-      | TermUb => ub
-      | TermRet r => Ret r
-      end.
+  terminates_in t tx.
 Proof.
-  intros Hterm Htr Hlater. pfold. rewrite /eqit_. induction Htr.
+  intros Hterm Htr. rewrite /terminates_in. induction Htr.
   - destruct tx; inversion Hterm. by constructor.
-  - destruct e as [e|e]; by destruct e.
+  - destruct e as [e|e]; destruct e, a.
+    constructor. apply IHHtr. destruct tx; by inversion Hterm.
   - destruct tx; inversion Hterm. destruct e as [e|e]; first by destruct e.
-    destruct e. constructor. by intros.
+    destruct e. constructor.
   - destruct tx; inversion Hterm.
-  - constructor; first done. by apply IHHtr.
+  - constructor. by apply IHHtr.
 Qed.
 
 Lemma execution n e σ tp' σ' κ tx :
@@ -1690,21 +1730,20 @@ Lemma execution n e σ tp' σ' κ tx :
   ∃ t1 t2 t3,
     (* TODO: consisting naming for interpretion relations *)
     (* TODO: abstraction for this composite relation *)
-    interleaves (R := val) 0 [v ← compile_expr false e ; step_if_not_val false e ;; Ret v]%itree t1 ∧
+    interleaves (R := val) 0 [v ← compile_expr e ; yield_if_not_val e ;; Ret v]%itree t1 ∧
     demonic_instantiates t1 t2 ∧
     eval σ t2 t3 ∧
     (* TODO: use UB adequacy *)
     match tx with
-    | TermUb => t3 ≈ ub
-    | TermRet r => ∃ σ', t3 ≈ Ret (σ', inl r)
+    | TermUb => terminates_in t3 TermUb
+    | TermRet r => ∃ σ', terminates_in t3 (TermRet (σ', inl r))
     end.
 Proof.
   intros Hsteps Hterm.
-  apply has_trace with (lt := false) (tx := tx) in Hsteps as (tid&tr&[Htinv Hstinv]&Htr); eauto.
+  apply has_trace with (tx := tx) in Hsteps as (tid&tr&[Htinv Hstinv]&Htr); eauto.
   rewrite /trace_invariant_state in Hstinv.
   destruct (interp_tr_state σ (interp_tr (sequencify tr))) as [tr'|] eqn:Heq;
     rewrite Heq // in Hstinv.
-  rewrite orb_false_r in Hstinv. 
   rewrite /trace_invariant_postfix in Htinv.
   rewrite Hterm in Htinv.
   apply interleaving_extending_trace in Htr as (t1&Hint&Htr).
@@ -1727,14 +1766,47 @@ Proof.
     eapply interp_tr_state_ub; last done. apply interp_tr_term. by apply sequencify_term in Htinv.
 Qed.
 
-Lemma execution_wpi' `{!invGS_gen hlc Σ} n e σ tp' σ' κ tx Φ :
+Lemma model_wpi {R} `{!invGS_gen hlc Σ} M n (tx : Terminal R) (Φ : R → iProp Σ) :
+  WPi (model_terminal n tx) @ laterH Identity ⊕ ubH ; M {{ Φ }} -∗
+  |={M}=> match tx with
+  | TermUb => False
+  | TermRet v => Φ v
+  end.
+Proof.
+  induction n; iIntros "Hwp".
+  - simpl. destruct tx.
+    * rewrite -wpi_ret' //.
+    * by iDestruct (wpi_ub with "Hwp") as "Hwp".
+  - iApply IHn. rewrite /= bind_vis -wpi_vis' /= wpi_clear_mask. by simpl_itree.
+Qed.
+
+Lemma model_wpi_later {R} `{!invGS_gen hlc Σ} M n (tx : Terminal R) (Φ : R → iProp Σ) :
+  WPi (model_terminal n tx) @ laterH Later ⊕ ubH ; M {{ Φ }} -∗
+  |={M}=> |={M}▷=>^n match tx with
+  | TermUb => False
+  | TermRet v => Φ v
+  end.
+Proof.
+  induction n; iIntros "Hwp".
+  - simpl. destruct tx.
+    * rewrite -wpi_ret' //.
+    * by iDestruct (wpi_ub with "Hwp") as "Hwp".
+  - iModIntro. simpl. iApply IHn. rewrite /= bind_vis -wpi_vis' /=. iMod "Hwp". simpl_itree.
+    (* TODO: Can't fill in this admitted proof because of a Coq crash. *)
+    iApply fupd_mask_intro; first admit. iIntros "Hfupd". iNext. simpl_itree.
+    iApply wpi_clear_mask. by iMod "Hfupd".
+Admitted.
+
+Lemma execution_wpi' `{!invGS_gen hlc Σ} m n e σ tp' σ' κ tx Φ :
   language.nsteps n ([e], σ) κ (tp', σ') →
   tp_termination tp' σ' = Some tx →
   state_interp σ -∗
-  WPi (v ← compile_expr false e; step_if_not_val false e;; Ret v) @ heaplangH ; ⊤ {{ Φ }} -∗
-  |={⊤}=> match tx with
-  | TermUb => False
-  | TermRet v => Φ v
+  WPi (v ← compile_expr e; yield_if_not_val e;; Ret v) @ heaplangH m ; ⊤ {{ Φ }} -∗
+  |={⊤}=> match (m, tx) with
+  | (Identity, TermUb) => False
+  | (Identity, TermRet v) => Φ v
+  | (Later, TermUb) => ∃ n, |={⊤}▷=>^n False
+  | (Later, TermRet v) => ∃ n, |={⊤}▷=>^n Φ v
   end.
 Proof.
   iIntros (Hstep Hstuck) "Hstate Hwp".
@@ -1743,24 +1815,38 @@ Proof.
   iDestruct (threadpool_adequacy with "Hwp") as "Hwp"; first apply Hint.
   iDestruct (demonicH_adequate with "Hwp") as "Hwp"; first apply Hinst.
   iDestruct (wpi_state with "Hstate Hwp") as "Hwp"; first apply Heval.
-  destruct tx.
-  - destruct Hterm as [σ'' Hterm]. rewrite Hterm -wpi_ret'. by iMod "Hwp" as "[_ HΦ]".
-  - rewrite Hterm /ub -wpi_vis' /=. by iMod "Hwp".
+  destruct tx, m.
+  - destruct Hterm as [σ'' [n' ->]%terminates_in_model].
+    iDestruct (model_wpi with "Hwp") as "Hwp".
+    by iMod "Hwp" as "[_ HΦ]".
+  - destruct Hterm as [σ'' [n' ->]%terminates_in_model].
+    iDestruct (model_wpi_later with "Hwp") as "Hwp".
+    iMod "Hwp". iModIntro. iExists n'. 
+    iApply step_fupdN_mono; last done. iIntros "[_ $]".
+  - apply terminates_in_model in Hterm as [n' ->].
+    by iDestruct (model_wpi with "Hwp") as "Hwp".
+  - apply terminates_in_model in Hterm as [n' ->].
+    iDestruct (model_wpi_later with "Hwp") as "Hwp".
+    iMod "Hwp". iModIntro. iExists n'. 
+    iApply step_fupdN_mono; last done. iIntros "$".
 Qed.
 
-Lemma ub_execution_wpi `{!invGS_gen hlc Σ} n e σ tp' σ' κ tx Φ :
+Lemma ub_execution_wpi `{!invGS_gen hlc Σ} m n e σ tp' σ' κ tx Φ :
   language.nsteps n ([e], σ) κ (tp', σ') →
   tp_termination tp' σ' = Some tx →
   state_interp σ -∗
-  WPi (compile_expr false e) @ heaplangH ; ⊤ {{ Φ }} -∗
-  |={⊤}=> match tx with
-  | TermUb => False
-  | TermRet v => Φ v
+  WPi (compile_expr e) @ heaplangH m ; ⊤ {{ Φ }} -∗
+  |={⊤}=> match (m, tx) with
+  | (Identity, TermUb) => False
+  | (Identity, TermRet v) => Φ v
+  | (Later, TermUb) => ∃ n, |={⊤}▷=>^n False
+  | (Later, TermRet v) => ∃ n, |={⊤}▷=>^n Φ v
   end.
 Proof.
   iIntros (Hstep Hterm) "Hstate Hwp".
   iApply (execution_wpi' with "Hstate"); eauto.
   iApply wpi_bind. iApply wpi_wand; last done.
-  iIntros (r) "HΦ". iApply wpi_bind. iApply @wpi_step_if_not_val.
-  by iApply @wpi_ret.
+  iIntros (r) "HΦ". iApply wpi_bind. rewrite /yield_if_not_val. destruct (to_val _).
+  - iApply wpi_ret. by iApply wpi_ret.
+  - iApply @wpi_yield. by iApply wpi_ret.
 Qed.
